Aesop/RuleTac/Basic.lean
@@ -44,8 +44,8 @@ Input for a rule tactic. Contains:
 structure RuleTacInput where
   goal : MVarId
   mvars : UnorderedArraySet MVarId
-  indexMatchLocations : HashSet IndexMatchLocation
-  patternInstantiations : HashSet RulePatternInstantiation
+  indexMatchLocations : Std.HashSet IndexMatchLocation
+  patternInstantiations : Std.HashSet RulePatternInstantiation
   options : Options'
   deriving Inhabited
 
