Aesop/Util/Basic.lean
@@ -42,7 +42,7 @@ def time' [Monad m] [MonadLiftT BaseIO m] (x : m Unit) : m Aesop.Nanos := do
 namespace HashSet
 
 -- TODO reuse old hash set instead of building a new one.
-def filter [BEq α] [Hashable α] (hs : HashSet α) (p : α → Bool) : HashSet α :=
+def filter [BEq α] [Hashable α] (hs : Std.HashSet α) (p : α → Bool) : Std.HashSet α :=
   hs.fold (init := ∅) λ hs a => if p a then hs.insert a else hs
 
 end HashSet
@@ -67,12 +67,12 @@ end PersistentHashSet
 -- TODO upstream; generalise to {m : Type u → Type v}.
 -- Need to generalise `HashMap.forM` first.
 scoped instance {m : Type u → Type u} [BEq α] [Hashable α] :
-    ForM m (HashMap α β) (α × β) where
+    ForM m (Std.HashMap α β) (α × β) where
   forM | m, f => m.forM λ a b => f (a, b)
 
 -- TODO upstream; generalise to {m : Type u → Type v}.
 scoped instance {m : Type u → Type u} [BEq α] [Hashable α] :
-    ForIn m (HashMap α β) (α × β) where
+    ForIn m (Std.HashMap α β) (α × β) where
   forIn := ForM.forIn
 
 section DiscrTree
@@ -218,7 +218,7 @@ def updateSimpEntryPriority (priority : Nat) (e : SimpEntry) : SimpEntry :=
   | .thm t => .thm { t with priority }
   | .toUnfoldThms .. | .toUnfold .. => e
 
-def getMVarDependencies (e : Expr) : MetaM (HashSet MVarId) := do
+def getMVarDependencies (e : Expr) : MetaM (Std.HashSet MVarId) := do
   let (_, deps) ←
     Lean.MVarId.getMVarDependencies.addMVars (includeDelayed := true) e
     |>.run {}
