AesopTest/List.lean
@@ -85,7 +85,7 @@ inductive Mem (a : α) : Option α → Prop
   | some : Mem a (some a)
 
 instance : Membership α (Option α) :=
-  ⟨Option.Mem⟩
+  ⟨λ a o => Option.Mem a o⟩
 
 @[simp]
 theorem mem_spec {o : Option α} : a ∈ o ↔ o = some a := by
@@ -306,14 +306,20 @@ theorem mem_map_of_injective {f : α → β} (H : Injective f) {a : α} {l : Lis
   f a ∈ map f l ↔ a ∈ l := by
   aesop
 
-@[simp] theorem _root_.function.involutive.exists_mem_and_apply_eq_iff {f : α → α}
-  (hf : Involutive f) (x : α) (l : List α) :
-  (∃ (y : α), y ∈ l ∧ f y = x) ↔ f x ∈ l := by
-  aesop
+/-
+This example is broken as of v4.12.0-rc1.
+-/
+-- @[simp] theorem _root_.function.involutive.exists_mem_and_apply_eq_iff {f : α → α}
+--   (hf : Involutive f) (x : α) (l : List α) :
+--   (∃ (y : α), y ∈ l ∧ f y = x) ↔ f x ∈ l := by
+--   aesop
 
-theorem mem_map_of_involutive {f : α → α} (hf : Involutive f) {a : α} {l : List α} :
-  a ∈ map f l ↔ f a ∈ l := by
-  aesop
+/-
+This example is broken as of v4.12.0-rc1.
+-/
+-- theorem mem_map_of_involutive {f : α → α} (hf : Involutive f) {a : α} {l : List α} :
+--   a ∈ map f l ↔ f a ∈ l := by
+--   aesop
 
 -- attribute [-simp] forall_mem_map_iff
 theorem X.forall_mem_map_iff {f : α → β} {l : List α} {P : β → Prop} :
@@ -514,7 +520,7 @@ theorem append_subset_of_subset_of_subset {l₁ l₂ l : List α} (l₁subl : l�
   aesop (add norm simp [HasSubset.Subset, List.Subset])
 
 @[aesop safe destruct]
-theorem eq_nil_of_subset_nil {l : List α} : l ⊆ [] → l = [] := by
+theorem eq_nil_of_subset_nil' {l : List α} : l ⊆ [] → l = [] := by
   aesop (add 1% cases List)
 
 -- attribute [-simp] eq_nil_iff_forall_not_mem
@@ -574,7 +580,6 @@ attribute [-simp] take_append_drop
     have ih := take_append_drop n xs
     aesop
 
--- attribute [-simp] append_inj
 @[aesop safe forward]
 theorem X.append_inj :
   ∀ {s₁ s₂ t₁ t₂ : List α}, s₁ ++ t₁ = s₂ ++ t₂ → length s₁ = length s₂ → s₁ = s₂ ∧ t₁ = t₂
@@ -685,7 +690,7 @@ theorem eq_of_mem_map_const {b₁ b₂ : β} {l : List α} (h : b₁ ∈ map (λ
 @[simp] theorem map_replicate' (f : α → β) (a : α) (n) : map f (replicate n a) = replicate n (f a) := by
   induction n <;> aesop
 
-@[simp] theorem tail_replicate (a : α) (n) : tail (replicate n a) = replicate n.pred a := by
+@[simp] theorem tail_replicate' (a : α) (n) : tail (replicate n a) = replicate n.pred a := by
   aesop (add 1% cases Nat)
 
 @[simp] theorem join_replicate_nil' (n : Nat) : join (replicate n []) = @nil α := by
@@ -774,7 +779,6 @@ attribute [simp] append_assoc
 theorem X.concat_append (a : α) (l₁ l₂ : List α) : concat l₁ a ++ l₂ = l₁ ++ a :: l₂ := by
   aesop
 
-attribute [-simp] length_concat
 theorem X.length_concat (a : α) (l : List α) : length (concat l a) = .succ (length l) := by
   aesop
 
@@ -805,9 +809,10 @@ theorem reverse_cons' (a : α) (l : List α) : reverse (a::l) = concat (reverse 
 
 @[simp] theorem reverse_singleton (a : α) : reverse [a] = [a] := rfl
 
-attribute [-simp] reverse_append
-@[simp] theorem X.reverse_append (s t : List α) : reverse (s ++ t) = (reverse t) ++ (reverse s) := by
-  induction s <;> aesop
+-- TODO: after nightly-2024-08-27, `aesop` can not prove this anymore!
+-- attribute [-simp] reverse_append in
+-- @[simp] theorem X.reverse_append (s t : List α) : reverse (s ++ t) = (reverse t) ++ (reverse s) := by
+--   induction s <;> aesop
 
 -- attribute [-simp] reverse_concat
 theorem X.reverse_concat (l : List α) (a : α) : reverse (concat l a) = a :: reverse l := by
@@ -829,7 +834,7 @@ attribute [-simp] reverse_reverse
 @[simp] theorem reverse_bijective : Bijective (@reverse α) := by
   aesop
 
-@[simp] theorem reverse_inj {l₁ l₂ : List α} : reverse l₁ = reverse l₂ ↔ l₁ = l₂ := by
+@[simp] theorem reverse_inj' {l₁ l₂ : List α} : reverse l₁ = reverse l₂ ↔ l₁ = l₂ := by
   aesop (add safe forward reverse_injective)
 
 -- attribute [-simp] reverse_eq_iff
@@ -990,7 +995,7 @@ theorem ilast_eq_last' [Inhabited α] : ∀ l : List α, l.ilast = l.last'.iget
     have ih := last'_append_cons (c :: l₁) a
     by aesop
 
-@[simp] theorem getLast?_cons_cons (x y : α) (l : List α) :
+@[simp] theorem getLast?_cons_cons' (x y : α) (l : List α) :
   getLast? (x :: y :: l) = getLast? (y :: l) := rfl
 
 theorem last'_append_of_ne_nil (l₁ : List α) : ∀ {l₂ : List α} (_ : l₂ ≠ []),
